examples/pseudo_bool/graph_encoding/compilation/max_common_induced_subgraphCompileScript.sml
@@ -1,0 +1,11 @@
+(*
+  Compiles the encoder
+*)
+open preamble compilationLib max_common_induced_subgraphProgTheory
+
+val _ = new_theory "max_common_induced_subgraphCompile"
+
+val max_common_induced_subgraph_compiled = save_thm("max_common_induced_subgraph_compiled",
+  compile_x64 "mcis" top_prog_def);
+
+val _ = export_theory ();
