examples/pseudo_bool/graph_encoding/max_common_induced_subgraphProgScript.sml
@@ -1,0 +1,215 @@
+(*
+  A simple (unverified) parse and printer
+*)
+open preamble basis max_common_induced_subgraphTheory;
+open cfLib basisFunctionsLib;
+
+val _ = new_theory "max_common_induced_subgraphProg";
+
+val _ = translation_extends "basisProg";
+
+(* Parser for LAD *)
+Definition blanks_def:
+  blanks (c:char) ⇔ c = #" " ∨ c = #"\n" ∨ c = #"\t" ∨ c = #"\r"
+End
+
+Definition tokenize_def:
+  tokenize (s:mlstring) =
+  case mlint$fromNatString s of
+    NONE => INL s
+  | SOME i => INR i
+End
+
+Definition toks_def:
+  toks s = MAP tokenize (tokens blanks s)
+End
+
+Definition parse_num_list_def:
+  (parse_num_list v [] acc = SOME (REVERSE acc)) ∧
+  (parse_num_list v (x::xs) acc =
+    case x of
+      INR (n:num) => parse_num_list v xs (n::acc)
+    | INL _ => NONE)
+End
+
+(* A parser for LAD format *)
+Definition parse_edges_def:
+  (parse_edges v i [] acc = SOME acc) ∧
+  (parse_edges v i (l::ls) acc =
+    case parse_num_list v l [] of
+      SOME (d::xs) =>
+        if LENGTH xs = d then parse_edges v (i+1) ls (insert i xs acc) else NONE
+    | _ => NONE)
+End
+
+Definition parse_lad_toks_def:
+  parse_lad_toks ls =
+  case ls of
+    [INR h]::rest =>
+      (case parse_edges h 0 rest LN of NONE => NONE
+      | SOME e => SOME (h,e))
+  | _ => NONE
+End
+
+(*
+val ladraw = ``[
+  strlit"5";
+  strlit"3 1 3 4";
+  strlit"3 0 3 4";
+  strlit"1 3";
+  strlit"3 0 1 2";
+  strlit"2 0 1";
+]``;
+
+val pattern = rconc (EVAL``THE (parse_lad_toks (MAP toks ^(ladraw)))``)
+
+val res = EVAL``MAP (pbc_string enc_string) (encode_full ^pattern ^pattern 1)``
+*)
+
+Definition usage_string_def:
+  usage_string = strlit "Usage: encode <LAD format file (pattern)> <LAD format file (target)>\n"
+End
+
+val r = translate usage_string_def;
+
+Definition notfound_string_def:
+  notfound_string f = concat[strlit"c Input file: ";f;strlit" no such file or directory\n"]
+End
+
+val r = translate notfound_string_def;
+
+val noparse_string_def = Define`
+  noparse_string f s = concat[strlit"c Input file: ";f;strlit" unable to parse in format: "; s;strlit"\n"]`;
+
+val r = translate noparse_string_def;
+
+val _ = translate blanks_def;
+val _ = translate tokenize_def;
+
+val _ = translate parse_num_list_def;
+val _ = translate insert_def;
+val _ = translate parse_edges_def;
+val _ = translate parse_lad_toks_def;
+
+val parse_lad = (append_prog o process_topdecs) `
+  fun parse_lad f =
+  (case TextIO.b_inputAllTokensFrom f blanks tokenize of
+    None => Inl (notfound_string f)
+  | Some lines =>
+  (case parse_lad_toks lines of
+    None => Inl (noparse_string f "LAD")
+  | Some x => Inr x))`
+
+val _ = translate k_size_def;
+val _ = translate has_mapping_def;
+val _ = translate all_has_mapping_def;
+val _ = translate one_one_def;
+val _ = translate all_one_one_def;
+val _ = translate lookup_def;
+val _ = translate graph_basicTheory.neighbours_def;
+
+Theorem is_edge_compute:
+  is_edge e a b =
+  case lookup a e of NONE => F
+  | SOME ns => MEMBER b ns
+Proof
+  simp[graph_basicTheory.is_edge_def]>>
+  every_case_tac>>metis_tac[MEMBER_INTRO]
+QED
+
+val _ = translate is_edge_compute;
+
+
+val _ = translate edge_map_def;
+
+val _ = translate COUNT_LIST_AUX_def;
+val _ = translate COUNT_LIST_compute;
+val _ = translate (graph_basicTheory.not_neighbours_def |> SIMP_RULE std_ss [MEMBER_INTRO]);
+val _ = translate not_edge_map_def;
+val _ = translate all_full_edge_map_def;
+
+val _ = translate encode_def;
+
+Definition log2_def:
+  log2 n =
+  if n < 2 then 0:num
+  else (log2 (n DIV 2))+1
+End
+
+val _ = translate log2_def;
+
+(* Just for the sake of translation *)
+Theorem LOG2_log2:
+  LOG 2 n = log2 n
+Proof
+  cheat
+QED
+
+val _ = translate pb_preconstraintFreeTheory.negate_def;
+val _ = translate iff_and_def;
+val _ = translate iff_or_def;
+val _ = translate walk_base_def;
+val _ = translate walk_aux_def;
+val _ = translate walk_ind_def;
+val _ = translate walk_k_def;
+
+val _ = translate (encode_connected_def |> SIMP_RULE std_ss [LOG2_log2])
+
+val _ = translate encode_full_def;
+
+Definition print_pbf_def:
+  print_pbf f = MAP (pbc_string enc_string) f
+End
+
+val res = translate pb_preconstraintFreeTheory.lit_string_def;
+val res = translate pb_preconstraintFreeTheory.lhs_string_def;
+val res = translate pb_preconstraintFreeTheory.pbc_string_def;
+val res = translate enc_string_def;
+val res = translate print_pbf_def;
+
+val _ = (append_prog o process_topdecs) `
+  fun print_list ls =
+    case ls of [] => () | (x::xs) => (print x; print"\n"; print_list xs)`
+
+val enc_and_print = (append_prog o process_topdecs) `
+  fun enc_and_print f1 f2 =
+  case parse_lad f1 of
+    Inl err => TextIO.output TextIO.stdErr err
+  | Inr pattern =>
+  (case parse_lad f2 of
+    Inl err => TextIO.output TextIO.stdErr err
+  | Inr target =>
+    print_list (print_pbf (encode_full pattern target 0))
+  )`
+
+val top = (append_prog o process_topdecs) `
+  fun top u =
+  case CommandLine.arguments () of
+    [f1,f2] => enc_and_print f1 f2
+  | _ => TextIO.output TextIO.stdErr usage_string`
+
+Theorem top_whole_prog_spec2:
+   hasFreeFD fs ⇒
+   whole_prog_spec2 top_v cl fs NONE (λfs'. ∃err. fs' = foo)
+Proof
+  cheat
+QED
+
+local
+
+val name = "top"
+val (sem_thm,prog_tm) =
+  whole_prog_thm (get_ml_prog_state()) name (UNDISCH top_whole_prog_spec2)
+val top_prog_def = Define`top_prog = ^prog_tm`;
+
+in
+
+Theorem top_semantics =
+  sem_thm
+  |> REWRITE_RULE[GSYM top_prog_def]
+  |> DISCH_ALL
+  |> SIMP_RULE(srw_ss())[GSYM CONJ_ASSOC,AND_IMP_INTRO];
+
+end
+
+val _ = export_theory();
